tests/lean/run/1051.lean
@@ -14,7 +14,6 @@ def SF.step [Monad m] (sa: as): SF as bs → SF' m as bs × bs
   (sf₁'.seq sf₂', sc)
 | fan => sorry
 
-
 def SF'.step [Monad m] (sa: as): SF' m as bs → SF'.{u} m as bs × bs
 | seq sf₁ sf₂ =>
   let (sf₁', sb) := sf₁.step sa
