tests/lean/run/structuralMutual.lean
@@ -453,7 +453,7 @@ error: failed to infer structural recursion:
 Cannot use parameter #2:
   its type is an inductive datatype and the datatype parameter
     n
-  which cannot be fixed as it is in a index, or depends on on index, and indices cannot be fixed parameters with structural recursion.
+  which cannot be fixed as it is an index or depends on an index, and indices cannot be fixed parameters when using structural recursion.
 -/
 #guard_msgs in
 def T.a {n : Nat} : T n n → Nat
